\section{Matrix representation of a su\-per\--anti\--auto\-mor\-phism}

In this section, we are going to express the super-anti-automorphism (not necessarily involutive) $\vphi$ in terms of matrices with entries in $\D$.
One could do that by following Equation \eqref{eq:vphi-r-Star-is-a-superconjugation}, but we will take a different path.

As before, we suppose $\D$ is a graded division superalgebra, $\U$ is a nonzero right graded module of finite rank over $\D$, $R = \End_\D (\U)$ and $\vphi$ is a degree-preserving super-anti-automorphism on $R$.
Also, let $\vphi_0$ be a super-anti-automorphism on $\D$ and $B$ be a nondegenerate $\vphi_0$-sesquilinear form on $\U$ determinig $\vphi$ as in Theorem \ref{thm:vphi-iff-vphi0-and-B}.

\begin{defi}\label{def:matrix-representing-B}
	Given a graded basis $\{e_1, \ldots, e_k\}$ of $\U$, the \emph{matrix representing the form $B$} is defined to be $\Phi = (\Phi_{ij}) \in M_k(\D)$, where $\Phi_{ij} = B(e_i, e_j)$.
\end{defi}

From now on, let $\mc B = \{e_1, \ldots, e_k\}$ be a fixed homogeneous $\D$-basis of $\U$, following Convention \ref{conv:pick-even-basis} (\ie, if $\D$ is odd, we take $\mc B$ with only even elements).
We will use $\mc B$ to identify $R = \End_\D (\U)$ with $M_k (\D)$.
Also, we will denote $|e_i|$ simply by $|i|$ for all $i \in \{1, \ldots, k\}$.

% We will assume that the even elements precede the odd ones. 

% We will also follow Convention \ref{conv:pick-even-basis}, \ie, if $\D$ is odd, we will choose the $\D$-basis $\mc B$ to be one having only even elements.

% \begin{convention}\label{conv:pick-even-basis}
% 	If $\D$ is odd (\ie, $\D\odd \neq 0$), we will choose the $\D$-basis $\mc B$ to be one having only even elements.
% 	This is possible because, given any homogeneous $\D$-basis, we can multiply its odd elements by a nonzero homogeneous odd element in $\D$.
% \end{convention}

\begin{remark}\label{rmk:M(D)=M(FF)-tensor-D}
	It is well know that we a natural isomorphism between $M_k(\D)$ and $M_k(\FF)\tensor \D$, where we use the usual tensor product of algebras.
	For superalgebras, though, we usually use a different product on the space $M_k(\FF)\tensor \D$, given by \[(r_1 \tensor s_1) (r_2 \tensor s_2) = \sign{r_2}{s_1} (r_1 r_2) \tensor (s_1 s_2).\]
	If we are following Convention \ref{conv:pick-even-basis}, either $M_k(\FF)$ or $\D$ have trivial canonical $\ZZ_2$-grading, hence both tensor products coincide.
\end{remark}

\begin{defi}
	Let $X = (x_{ij})$ be a matrix in $M_k (\D)$.
	We define $\vphi_0 (X)$ to be the matrix obtained by applying $\vphi_0$ in each entry, \ie, $\vphi_0 (X) \coloneqq (\vphi_0(x_{ij}))$.
	We also extend the definition \emph{supertranspose} {(\tt see ??)} to matrices over $\D$ by putting $X\stransp \coloneqq \big((-1)^{(|i| + |j|) |i|} x_{ji} \big)$.
	Note that, with our choice of $\mc B$ in the case of odd $\D$, we have that $X\stransp = X\transp$, the ordinary transpose.
\end{defi}

\begin{prop}\label{prop:matrix-vphi}
	Let $\Phi$ be the matrix representing $B$.
	For every $r\in  R\even \cup R\odd$, let $X \in M_k(\D)$ be the matrix representing $r$ and let $Y \in M_k(\D)$ be the matrix representing $\vphi(r)$.
	Then, following Conventions \ref{conv:pick-even-form} and \ref{conv:pick-even-basis}, we have that
	%
	\begin{align}
		Y & = \Phi\inv\, \vphi_0( X\stransp )\, \Phi. \addtocounter{equation}{1}\tag{\theequation}\label{eq:matrix-vphi-D-even}
		\intertext{and, if $\D$ is odd, we have}
		Y & = \sign{B}{r}\,\Phi\inv\, \vphi_0( X\stransp )\, \Phi.\addtocounter{equation}{1}\tag{\theequation}\label{eq:matrix-vphi-D-odd}
	\end{align}
\end{prop}

\begin{proof}
	First of all, note that Equation \eqref{eq:superadjunction} is equivalent to the following:
	%
	\begin{alignat*}{2}
		\forall e_i, e_j \in \mc B, &  & B(re_i, e_j)                                              & = \sign{r}{i} B(e_i, \vphi(r) e_j),
		\intertext{which, by the definitions of $X$, $Y$ and $\Phi$, becomes}
		\forall e_i, e_j \in \mc B, &  & \quad B\bigg(\sum_{\ell=1}^k e_\ell x_{\ell i}, e_j\bigg) & = \sign{r}{i} B\bigg(e_i, \sum_{\ell=1}^k e_\ell y_{\ell j}\bigg) \addtocounter{equation}{1}\tag{\theequation}\label{eq:superadjunction-matrix}.
	\end{alignat*}
	%

	Fix arbitrary $p,q \in \{1, \ldots, k\}$ and suppose that the $(p,q)$-entry of $X$ is a nonzero $G^\#$-homogeneous element of $\D$ and $x_{ij} = 0$ elsewhere, \ie, $X$ represents the map $r \in \End_\D(\U)$ defined by $r e_i = \delta_{iq} e_p x_{pq}$.
	By the $\FF$-linearity of Equation \eqref{eq:matrix-vphi-D-even} %and \eqref{eq:matrix-vphi-D-odd}
	, it suffices to consider such $X$.
	Note that $|r| = |e_p| + |x_{pq}| - |e_q| = |p| + |q| + |x_{pq}|$.
	Then, on the one hand,
	%
	\begin{align*}
		B\bigg(\sum_{\ell=1}^k e_\ell x_{\ell i}, e_j\bigg) = B (e_p x_{pi}, e_j) & = (-1)^{ (|B| + |p|) |x_{pi}|} \vphi_0(x_{pi}) B(e_p, e_j)
		\\&= (-1)^{ (|B| + |p|) |x_{pi}|} \vphi_0(x_{pi}) \Phi_{pj},
		%\end{align*}
		%
		\intertext{which is only nonzero if $i = q$. On the other hand,}
		%
		%\begin{align*}
		\sign{r}{i} B\bigg(e_i, \sum_{\ell=1}^k e_\ell y_{\ell j}\bigg)
		                                                                          & = \sign{r}{i} \sum_{\ell=1}^k B(e_i, e_\ell) y_{\ell j}                                                                                           \\
		                                                                          & = (-1)^{ (|p| + |q| + |x_{pq}|) |i| } \sum_{\ell=1}^k \Phi_{i \ell} y_{\ell j}.
		%\end{align*}
		%
		\intertext{Therefore, Equation \eqref{eq:superadjunction-matrix} is equivalent to, for all $i,j \in \{1, \ldots, k\}$,}
		%
		%\begin{align*}
		(-1)^{ (|B| + |p|) |x_{pi}|} \vphi_0(x_{pi}) \Phi_{pj} %&= \sign{r}{i} \sum_{\ell=1}^k \Phi_{i \ell} y_{\ell j}\\
		                                                                          & = (-1)^{ (|p| + |q| + |x_{pq}|) |i| } \sum_{\ell=1}^k \Phi_{i \ell} y_{\ell j}. \addtocounter{equation}{1}\tag{\theequation}\label{eq:expression}
	\end{align*}
	%

	If $\D$ is even, then $|x_{pi}| = \bar 0$ and this equation reduces to
	\[              \vphi_0(x_{pi}) \Phi_{pj} = (-1)^{ (|p| + |q|) |i| } \sum_{\ell=1}^k \Phi_{i \ell} y_{\ell j}
	\]
	or, equivalently,
	\[
		\sum_{\ell=1}^k \Phi_{i \ell} y_{\ell j} = (-1)^{ (|p| + |q|) |i| } \vphi_0(x_{pi}) \Phi_{pj}.
	\]
	The left-hand side is the $(i,j)$-entry of $\Phi\, Y$.
	The right-hand side is only nonzero if $i = q$, so it can be rewritten as
	$(-1)^{ (|p| + |i|) |i| } \vphi_0(x_{pi}) \Phi_{pj}$.
	Recalling our choice of $X$, this is equal to $\sum_{\ell =1}^k (-1)^{ (|\ell| + |i|) |i| } \vphi_0(x_{\ell i}) \Phi_{\ell j}$, since $x_{\ell i}$ is only nonzero if $\ell = p$.
	Hence the right-hand side is the $(i,j)$-entry of $\vphi_0 (X\stransp) \Phi$, and Equation \eqref{eq:matrix-vphi-D-even} follows.

	If $\D$ is odd, by our choice of basis, Equation \eqref{eq:expression} reduces to
	\[
		(-1)^{|B| |x_{pi}|} \vphi_0(x_{pi}) \Phi_{pj} =  \sum_{\ell=1}^k \Phi_{i \ell} y_{\ell j},
	\]
	which, by the same reasoning as above, implies $(-1)^{|B||r|} \vphi_0(X\stransp) \Phi = \Phi Y$. 
% 	But we are following Convention \ref{conv:pick-even-form}, hence $|B| = \bar 0$ and, therefore, we have the desired result.
\end{proof}

% \begin{proof}
%     First of all, note that Equation \ref{eq:superadjunction} is equivalent to, for all $e_i, e_j \in \mc B$,
%     %
%     \[
%         B(re_i, e_j) = \sign{r}{i} B(e_i, \vphi(r) e_j).
%     \]
%     By the definitions of $X$, $Y$ and $\Phi$, we have that
%     %
%     \begin{align*}
%         B\bigg(\sum_{\ell=1}^k e_\ell x_{\ell i}, e_j\bigg) &= \sum_{\ell=1}^k (-1)^{( |B| + |\ell|) |x_{\ell i}|} \vphi_0( x_{\ell i} ) B (e_\ell x_{\ell i}, e_j)\\ &= \sum_{\ell=1}^k (-1)^{( |B| + |\ell|) |x_{\ell i}|} \vphi_0( x_{\ell i} ) \Phi_{\ell j}
%         \intertext{and}
%         \sign{r}{i} B\bigg(e_i, \sum_{\ell=1}^k e_\ell y_{\ell j}\bigg) 
%         &= \sign{r}{i} \sum_{\ell=1}^k B(e_i, e_\ell) y_{\ell j}\\
%         &= \sign{r}{i} \sum_{\ell=1}^k \Phi_{i \ell} y_{\ell j}. 
%     \end{align*}
%     %

%     Let $p,q \in \{1, \ldots, k\}$, and suppose $X$ is such that $x_{pq}$ is a nonzero $G^\#$-homogeneous element of $\D$ and $x_{ij} = 0$ elsewhere, \ie, $X$ represents the map $r \in \End_\D(\U)$ defined by $r e_i = \delta_{iq} e_p x_{pq}$. 
%     By the $\FF$-linearity of Equations \eqref{eq:matrix-vphi-D-even} and \eqref{eq:matrix-vphi-D-odd}, it suffices to consider such $X$. 
%     Note that $|r| = |e_q| + |x_{pq}| - |e_p| = |p| + |q| + |x_{pq}|$. 
%     Then
%     %
%     \begin{align*}
%         B\bigg(\sum_{\ell=1}^k e_\ell x_{\ell i}, e_j\bigg) = B (e_p x_{pi}, e_j) &= (-1)^{ (|B| + |p|) |x_{pi}|} \vphi_0(x_{pi}) B(e_p, e_j)
%         \\&= (-1)^{ (|B| + |p|) |x_{pi}|} \vphi_0(x_{pi}) \Phi_{pj},
%     \end{align*}
%     %
%     which is only nonzero if $i = q$. 
%     Combining this with Equation \eqref{eq:superadjunction-matrix}, we get
%     %
%     \begin{align*}
%         (-1)^{ (|B| + |p|) |x_{pi}|} \vphi_0(x_{pi}) \Phi_{pj} &= \sign{r}{i} \sum_{\ell=1}^k \Phi_{i \ell} y_{\ell j}\\
%         &= (-1)^{ (|p| + |q| + |x_{pq}|) |i| } \sum_{\ell=1}^k \Phi_{i \ell} y_{\ell j}. \addtocounter{equation}{1}\tag{\theequation}\label{eq:expression}
%     \end{align*}
%     %
%     If $\D$ is even, then $|x_{pi}| = 0$ and this expression reduces to
%     \[              \vphi_0(x_{pi}) \Phi_{pj} = (-1)^{ (|p| + |q|) |i| } \sum_{\ell=1}^k \Phi_{i \ell} y_{\ell j}
%     \]
%     or, reordering it, 
%     \[
%         \sum_{\ell=1}^k \Phi_{i \ell} y_{\ell j} = (-1)^{ (|p| + |q|) |i| } \vphi_0(x_{pi}) \Phi_{pj}.
%     \]
%     The left-hand side is the entry $ij$ of $\Phi\, Y$. 
%     The right-hand side is only nonzero if $i = q$, so it can be rewritten as 
%     $(-1)^{ (|p| + |i|) |i| } \vphi_0(x_{pi}) \Phi_{pj}$. 
%     Also, recalling our choice of $X$, it is equal to $\sum_{\ell =1}^k (-1)^{ (|\ell| + |i|) |i| } \vphi_0(x_{\ell i}) \Phi_{\ell j}$, since $x_{\ell i}$ is only nonzero if $\ell = p$. Hence the right-hand side is the $ij$ entry of $\vphi_0 (X\stransp) \Phi$, and Equation \eqref{eq:matrix-vphi-D-even} follows. 

%     If $\D$ is odd, by our choice of basis, Equation \eqref{eq:expression} reduces to
%     \[
%         (-1)^{|B| |x_{pi}|} \vphi_0(x_{pi}) \Phi_{pj} =  \sum_{\ell=1}^k \Phi_{i \ell} y_{\ell j},
%     \]
%     which implies $(-1)^{|B||r|} \phi_0(X\stransp) \Phi = \Phi Y$.
% \end{proof}

% \begin{remark}
%     Note that if $\D$ is odd, replacing $B$ by $dB$ with an odd $d$ if necessary, we can guarantee that $B$ is even. 
%     In this case, Equation \eqref{eq:matrix-vphi-D-odd} reduces to \eqref{eq:matrix-vphi-D-even}.
% \end{remark}

% \begin{cor}[of the proof]
%     Let $\vphi_0$ be a super-anti-automorphism on $\D$ and let $B$ be a nonzero $\vphi_0$-sesquilinear form on $\U$. If $\vphi\from R \to R$ be a parity preserving map satisfying Equation \eqref{eq:superadjunction}. 
%     Then $B$ is nondegenerate if, and only if, $\vphi$ is a super-anti-automorphism.
% \end{cor}
